decide to stay with current model because the issue was not restricting the structure by another theorem. We add an iff and other changes are just correcting after this change

model.v
@@ -6,7 +6,7 @@ Require Import RelationClasses.
 From Paco Require Import paco.
 From mathcomp Require Import all_ssreflect.
 From mathcomp Require Import order.
-Require Import Stdlib.Streams.Streams.
+Require Import Coq.Lists.Streams.
 From HB Require Import structures.
 From deriving Require Import deriving.
 Require Import Coq.Program.Equality.
@@ -80,8 +80,9 @@ Record myrel (A : Set) :=
                              forall a0 a1, rel l1 a0 a1 -> rel l0 a0 a1;
            _ : forall l0 l1, order l0 l1 ->
                              forall a, dis l1 a -> dis l0 a;
-           _: forall l a0 a1, dis l a0 -> rel l a0 a1 -> dis l a1
-
+           _: forall l a0, dis l a0 -> forall a1, dis l a1 <-> rel l a0 a1 (* dis is an equivalence class: (->) contains enough, (<-) does not include too much s  *)
+(*           _: forall l a0 a1, dis l a0 -> rel l a0 a1 -> dis l a1;
+           _: forall l a0 a1, dis l a0 -> dis l a1 -> rel l a0 a1*)
           }.
 
 (*Existing Class myrel. 
@@ -159,10 +160,6 @@ Notation "[ i ]" := (interp i).
 
 
 
-Check nat.
-
-
-
 (** Process type **)
 Inductive Proc : Ty -> Ty -> Type :=
 | out  : forall {I O : Ty}, interp O -> Proc I O  
@@ -178,10 +175,9 @@ Derive NoConfusionHom for Proc.
 Derive Signature for Proc.
 
 Definition xor (b1 b2 : bool) := (Datatypes.negb (b1 == b2)).
-Arguments out I O o.
 
 Inductive reduceI : forall (I O : Ty), Proc I O -> interp I -> Proc I O -> Prop :=
-| reduce_outI I O i (o : [O]) : reduceI (@out I _ o) i (@out I _ o)
+| reduce_outI I O i (o : [O]) : reduceI ( @out I _ o) i ( @out I _ o)
 | reduce_mapI (I I' O O' : Ty) p p' i i' (f : [I] -> [I']) (g : [O] -> [O']) : f i = i' -> reduceI p i' p' -> reduceI (map f g p) i (map f g p')
 | reduce_staI (V I O : Ty) v v' (p : Proc (Times V I) O) p' i (f : [I] -> [V] -> [V]) (g : [O] -> [V] -> [V]) : f i v = v' -> reduceI p (v', i) p' -> reduceI (sta f g v p) i (sta f g v' p')
 | reduce_swiI (I O : Ty) b b' b'' (p : Proc I (Times Bool O)) p' (i : [I]) : b'' = xor b b' -> reduceI p i p' -> reduceI (swi b p) (b', i) (swi b'' p')
@@ -196,7 +192,7 @@ Hint Constructors reduceI : core.
 Hint Resolve reduce_mapI reduce_staI reduce_swiI reduce_maybeI reduce_maybeI2 reduce_parI reduce_loopI : omitdb.*)
 
 Inductive reduceO : forall (I O : Ty), Proc I O -> [O] -> Proc I O -> Prop :=
-| reduce_outO (I O : Ty) (o : [O]) : reduceO (@out I _ o) o (@out I _ o)
+| reduce_outO (I O : Ty) (o : [O]) : reduceO ( @out I _ o) o ( @out I _ o)
 | reduce_mapO (I I' O O' : Ty) p p' o o' (f : [I] -> [I']) (g : [O] -> [O']) : g o = o' -> reduceO p o p' -> reduceO (map f g p) o' (map f g p')
 | reduce_staO (V I O : Ty) v v' p p' o (f : [I] -> [V] -> [V]) (g : [O] -> [V] -> [V]) : g o v = v' -> reduceO p o p' -> reduceO (sta f g v p) (v', o) (sta f g v' p')
 | reduce_swiO (I O : Ty) (p : Proc I (Times Bool O)): reduceO (swi false p) None (swi false p)
@@ -209,12 +205,15 @@ Hint Constructors reduceO : core.
 Ltac check_if_var x :=
   first [ is_var x;fail 1 "Term" x "is not a bare variable" | idtac ].
 
-Ltac match_dd := 
-   repeat
+Ltac match_dd_once := 
     match goal with
     | H : reduceI ?p _ _ |- _ => check_if_var p; dependent destruction  H
     | H : reduceO ?p _ _ |- _ => check_if_var p; dependent destruction  H
     end.
+
+
+Ltac match_dd := 
+   repeat match_dd_once.
 
 (*Hint Resolve reduce_mapO reduce_staO reduce_swiO reduce_swiO2 reduce_maybeO reduce_parO reduce_loopO : omitdb.*)
 
@@ -246,15 +245,11 @@ Definition MapS  (I I' O O' : Ty) (f : [I] -> [I']) (g : [O] -> [O']) s s' := pa
 
 Definition MapRel (I I' O O' : Ty) (f : [I] -> [I']) (g : [O] -> [O']) s p := exists s', MapS f g s' s /\ trace s' p.
 
-Lemma TraceLemma : forall (I I' O O' : Ty) (f : [I] -> [I']) (g : [O] -> [O']) s p, MapRel f g s p -> TraceF (MapRel f g) s p.
 
 
-Lemma MapSP : forall (I I' O O' : Ty) (f : [I] -> [I']) (g : [O] -> [O']) s p, trace s (map f g p) -> exists s', MapS f g s' s /\ trace s' p.
-Proof.
+(*Lemma MapSP : forall (I I' O O' : Ty) (f : [I] -> [I']) (g : [O] -> [O']) s p, trace s (map f g p) -> exists s', MapS f g s' s /\ trace s' p.
+Proof.*)
 
-
-
-  
 Definition publicRel (A : Ty) : myrel ([A]).
   refine (@MyRel _
             (fun l b => False)
@@ -267,6 +262,7 @@ intros.
 done.
 eauto.
 eauto.
+intros. done.
 Defined.
 
 Definition toPublicRel (A : Ty) (ARel : myrel [A]) : myrel ([A]).
@@ -280,32 +276,55 @@ Definition toPublicRel (A : Ty) (ARel : myrel [A]) : myrel ([A]).
 intros. all: de ARel. eauto.
 Defined.
 
+Lemma order_bot : forall (l : level), order l \bot -> l = \bot.
+Proof.
+intros.
+rewrite /order lex0 in H.
+by apply/eqP.
+Qed.
+
+
+Lemma not_booleq : forall (A : eqType) (a : A), a != a -> False.
+Proof.
+intros.
+move/eqP : H.
+done.
+Qed.
+Hint Resolve not_booleq.
+
+
+  
 Definition semiprivateRel (A : Ty) : myrel ([A]).
   refine (@MyRel _
-            (fun l b => if l == \bot then True else False)
-            (fun l b1 b2 => b1 = b2)
+            (fun l b => l = \bot)
+            (fun l b1 b2 => b1 = b2 \/ l = \bot)
             _
             _
             _
             _).
+  - intros l. con. 
+    + intro. auto. 
+    + intros x y. case. auto.
+      intros. subst. auto.
+      rewrite /Transitive.
+      intros. de H. de H0. subst.
+      auto.
+intros.      
+de H0.
+subst.
+move/order_bot : H.
+move=>->. auto.
 intros.
-done.
-intros. de (eqVneq l1 \bot). rewrite /order in H. subst. rewrite lex0 in H. rewrite H. done.
-eauto.
+subst.
+move/order_bot : H.
+move=>->. done.
+intros.
+subst.
+con.
+auto.
+auto.
 Defined.
 
-Definition privateRel (A : Ty) : myrel ([A]).
-  refine (@MyRel _
-            (fun l b => True)
-            (fun l b1 b2 => b1 = b2)
-            _
-            _
-            _
-            _).
-intros.
-done. done.
-eauto.
-Defined.
 
 Definition Clause1 (I O : Ty) (l : level) (IRel : myrel [I]) (ORel : myrel [O]) (R : Stream ([I] + [O]) -> Proc I O -> Prop) s p : Prop :=
   forall i s', s = (Cons (inl i) s') -> dis IRel l i -> R s' p.
@@ -437,7 +456,11 @@ Definition eqpair {I O : Ty} (IRel : myrel [I]) (ORel : myrel [O]) : myrel ([Tim
   - move=> l0 l1 HOrder a0 a1 [] HI HO.
     destruct IRel,ORel;ssa. eauto. eauto.
 
-  - eauto. eauto.
+  - eauto.
+
+    intros. con.
+done.
+done.
 Defined.
 
 Definition eqpair_LR {I O : Ty} (IRel : myrel [I]) (ORel : myrel [O]) : myrel ([Times I O]).
@@ -468,13 +491,17 @@ Definition eqpair_LR {I O : Ty} (IRel : myrel [I]) (ORel : myrel [O]) : myrel ([
     destruct IRel,ORel;ssa. eauto. eauto.
 
   - intros. ssa. de IRel. eauto. de ORel. eauto.
-  - intros. ssa. de IRel. eauto. de ORel. eauto.
+  - intros. ssa. de IRel. con.
+    ssa. apply/i;eauto.
+    de ORel. apply/i0;eauto.
+    ssa. apply/i;eauto.
+    de ORel. apply/i0;eauto.
 Defined.
 
 Definition eqpair_L {I O : Ty} (IRel : myrel [I]) (ORel : myrel [O]) : myrel ([Times I O]).
   refine (@MyRel _ 
             (fun (l : level) io => dis IRel l (fst io))
-            (fun l io1 io2 => rel IRel l (fst io1) (fst io2) /\ rel ORel l (snd io1) (snd io2))
+            (fun l io1 io2 => rel IRel l (fst io1) (fst io2) /\ rel ORel l (snd io1) (snd io2) \/ dis IRel l (fst io1) /\ dis IRel l (fst io2))
             _
             _
             _
@@ -483,29 +510,51 @@ Definition eqpair_L {I O : Ty} (IRel : myrel [I]) (ORel : myrel [O]) : myrel ([T
     con. destruct IRel. destruct ORel. simpl. con.
     move: (equiv0 l). case. eauto.
     move: (equiv1 l). case. eauto.
-  - con. destruct H. destruct IRel. destruct ORel. simpl. 
+  - rewrite /Symmetric. intros. destruct H. destruct IRel. destruct ORel. simpl.
+    ssa. left.
     move: (equiv0 l). case.
-    move => _ Hsym _.  apply Hsym. eauto.
+    move => _ Hsym _. con.  apply Hsym. eauto.
 
-    destruct H. destruct IRel. destruct ORel. simpl. 
-    move: (equiv1 l). case. eauto.
+    move: (equiv1 l). case.
+    move => _ Hsym' _.  apply Hsym'. eauto.
 
-  - destruct IRel,ORel. simpl. con.
-    ssa. move: (equiv0 l). case. move=> _ _ Htrans. eauto.
-    ssa. move: (equiv1 l). case. move=> _ _ Htrans. eauto.
+    ssa.
+
+  - destruct IRel,ORel. simpl. intro. intros.
+
+    de H. de H0. left. ssa.
+    move: (equiv0 l). case. move=> _ _ Htrans. eauto.
+    move: (equiv1 l). case. move=> _ _ Htrans. eauto.
+
+    right. ssa. apply/i. apply: H0.
+    move: (equiv0 l). case.
+    move=> _ Hsym _. apply/Hsym. done.
+
+    de H0.
+
+    right. ssa. apply/i. apply: H1. done.
 
 
-  - move=> l0 l1 HOrder a0 a1 [] HI HO.
-    destruct IRel,ORel;ssa. eauto. eauto.
+  - intros. de H0.
+    left.
+    de IRel;eauto.
+    de ORel;eauto.
+    right.
+    de IRel;eauto.
 
-  - intros. de IRel;de ORel. eauto.
-  - intros. de IRel;de ORel. eauto.
+  - intros. de IRel;eauto.
+
+  - intros. con.
+    intros. eauto.
+    case. case. move=> HH _.
+    de IRel;eauto. apply/i. 2:eauto. done.
+    ssa.
 Defined.
 
 Definition eqpair_R {I O : Ty} (IRel : myrel [I]) (ORel : myrel [O]) : myrel ([Times I O]).
   refine (@MyRel _ 
             (fun (l : level) io => dis ORel l (snd io))
-            (fun l io1 io2 => rel IRel l (fst io1) (fst io2) /\ rel ORel l (snd io1) (snd io2))
+            (fun l io1 io2 => rel IRel l (fst io1) (fst io2) /\ rel ORel l (snd io1) (snd io2) \/ dis ORel l (snd io1) /\ dis ORel l (snd io2))
             _
             _
             _
@@ -514,29 +563,72 @@ Definition eqpair_R {I O : Ty} (IRel : myrel [I]) (ORel : myrel [O]) : myrel ([T
     con. destruct IRel. destruct ORel. simpl. con.
     move: (equiv0 l). case. eauto.
     move: (equiv1 l). case. eauto.
-  - con. destruct H. destruct IRel. destruct ORel. simpl. 
+  - rewrite /Symmetric. intros. destruct H. destruct IRel. destruct ORel. simpl.
+    ssa. left.
     move: (equiv0 l). case.
-    move => _ Hsym _.  apply Hsym. eauto.
+    move => _ Hsym _. con.  apply Hsym. eauto.
 
-    destruct H. destruct IRel. destruct ORel. simpl. 
-    move: (equiv1 l). case. eauto.
+    move: (equiv1 l). case.
+    move => _ Hsym' _.  apply Hsym'. eauto.
 
-  - destruct IRel,ORel. simpl. con.
-    ssa. move: (equiv0 l). case. move=> _ _ Htrans. eauto.
-    ssa. move: (equiv1 l). case. move=> _ _ Htrans. eauto.
+    ssa.
+
+  - destruct IRel,ORel. simpl. intro. intros.
+
+    de H. de H0. left. ssa.
+    move: (equiv0 l). case. move=> _ _ Htrans. eauto.
+    move: (equiv1 l). case. move=> _ _ Htrans. eauto.
+
+    right. ssa. apply/i0. apply: H0.
+    move: (equiv1 l). case.
+    move=> _ Hsym _. apply/Hsym. done.
+
+    de H0.
+
+    right. ssa. apply/i0. apply: H1. done.
 
 
-  - move=> l0 l1 HOrder a0 a1 [] HI HO.
-    destruct IRel,ORel;ssa. eauto. eauto.
+  - intros. de H0.
+    left.
+    de IRel;eauto.
+    de ORel;eauto.
+    right.
+    de IRel;eauto.
 
-  - intros. de IRel;de ORel. eauto.
-  - intros. de IRel;de ORel. eauto.
+  - intros. de ORel;eauto. de ORel;eauto.
+
+  - intros. de ORel;eauto.
+    intros. con. ssa.
+    case. case. intros. de ORel. apply/i. 2:eauto. done.
+    case. ssa.
 Defined.
+
+Lemma dis_rel_dis : forall (I : Ty) (IRel : myrel [I]) l x y, dis IRel l x -> rel IRel l x y -> dis IRel l y.
+Proof.
+  intros. de IRel. apply/i;eauto.
+Qed.
+Lemma dis_rel_dis2 : forall (I : Ty) (IRel : myrel [I]) l x y, dis IRel l x -> rel IRel l y x -> dis IRel l y.
+Proof.
+  intros. de IRel. apply/i;eauto.
+  move:(equiv0 l)=> [] _ Hsym _. apply/Hsym. auto.
+Qed.
+Lemma dis_dis_rel : forall (I : Ty) (IRel : myrel [I]) l x y, dis IRel l x -> dis IRel l y -> rel IRel l x y.
+Proof.
+  intros. de IRel;eauto. apply/i;eauto.
+Qed.
+
+
+Hint Resolve dis_rel_dis dis_rel_dis2 dis_dis_rel.
+
+
 
 Definition eqpair_OR {I O : Ty} (IRel : myrel [I]) (ORel : myrel [O]) : myrel ([Times I O]).
   refine (@MyRel _ 
             (fun (l : level) io => dis IRel l (fst io) \/ dis ORel l (snd io))
-            (fun l io1 io2 => rel IRel l (fst io1) (fst io2) /\ rel ORel l (snd io1) (snd io2))
+            (fun l io1 io2 => rel IRel l (fst io1) (fst io2) /\ rel ORel l (snd io1) (snd io2) \/
+                                (dis IRel l (fst io1) \/ dis ORel l (snd io1)) /\
+                                (dis IRel l (fst io2) \/ dis ORel l (snd io2))                                  
+            )
             _
             _
             _
@@ -545,30 +637,52 @@ Definition eqpair_OR {I O : Ty} (IRel : myrel [I]) (ORel : myrel [O]) : myrel ([
     con. destruct IRel. destruct ORel. simpl. con.
     move: (equiv0 l). case. eauto.
     move: (equiv1 l). case. eauto.
-  - con. destruct H. destruct IRel. destruct ORel. simpl. 
-    move: (equiv0 l). case.
-    move => _ Hsym _.  apply Hsym. eauto.
+  - intro. intros. destruct H.
+    left. destruct IRel,ORel. simpl in *.
+    destruct H.
+    con.
+    move: (equiv0 l)=> [] _ Hsym _.
+    apply/Hsym. done.
+    move: (equiv1 l)=> [] _ Hsym _.
+    apply/Hsym. done. ssa.
 
-    destruct H. destruct IRel. destruct ORel. simpl. 
-    move: (equiv1 l). case. eauto.
+    
+    intro. intros.
+    de H.
+    * de H0.
+      ** left. con.
+         de IRel. move: (equiv0 l)=>[] _ _ Htrans. apply/Htrans;eauto.
+         de ORel. move: (equiv0 l)=>[] _ _ Htrans. apply/Htrans;eauto.    
+      ** de H0. have: dis IRel l x.1 by eauto. move=>HH.
+         right. con. auto. auto.
+         have: dis ORel l x.2 by eauto. move=>HH.
+         right. con. auto. auto.
+    * de H0. right. con. auto.
+      de H1. eauto. eauto.
 
-  - destruct IRel,ORel. simpl. con.
-    ssa. move: (equiv0 l). case. move=> _ _ Htrans. eauto.
-    ssa. move: (equiv1 l). case. move=> _ _ Htrans. eauto.
+
+      intros. destruct H0.
+      ** left. destruct IRel. destruct ORel. simpl in *. ssa;eauto.
+      ** right. destruct IRel. destruct ORel. simpl in *. ssa;eauto.
+         de H0;eauto. de H1;eauto.
 
 
-  - move=> l0 l1 HOrder a0 a1 [] HI HO.
-    destruct IRel,ORel;ssa. eauto. eauto.
+         intros. destruct IRel. destruct ORel. simpl in *.
+         destruct H0;eauto.
 
-  - intros. de H0. de IRel. eauto. 
-  - intros. de ORel. eauto.
-  - intros. ssa. de IRel. de ORel. de H. eauto. eauto.
+
+         intros. con. intros. de H.
+         case. case. intros. de H. eauto. eauto.
+         de H.
 Defined.
 
 Lemma eqsum {I O : Ty} (IRel : myrel [I]) (ORel : myrel [O]) : myrel ([Sum I O]).
   refine (@MyRel _ 
             (fun (l : level) io => match io with | inl i => dis IRel l i | inr o => dis ORel l o end)
-            (fun l io1 io2 => match io1,io2 with | inl i1,inl i2 => rel IRel l i1 i2 | inr o1,inr o2 => rel ORel l o1 o2 | _,_ => False end)
+            (fun l io1 io2 => match io1,io2 with | inl i1,inl i2 => rel IRel l i1 i2
+                                            | inr o1,inr o2 => rel ORel l o1 o2
+                                            | inl i1, inr i2 => dis IRel l i1 /\ dis ORel l i2
+                                            | inr i1, inl i2 => dis ORel l i1 /\ dis IRel l i2 end)
             _
             _
             _
@@ -587,18 +701,31 @@ Lemma eqsum {I O : Ty} (IRel : myrel [I]) (ORel : myrel [O]) : myrel ([Sum I O])
 
     destruct IRel. destruct ORel. simpl.
     intro. ssa. de x. de y. de z.
-    move: (equiv0 l). case. eauto. de y. de z. 
+    move: (equiv0 l). case. eauto. apply/i. 2:eauto.
     move: (equiv1 l). case. eauto.
 
+    move: (equiv0 l). case. eauto. 
+    de z. apply/i. done. done.
+    apply/i0. eauto.
+    done.
+    de y. de z. apply/i. 2:eauto. done.
+    apply/i0. done. done.
+    de z. apply/i0. eauto.
+    move:(equiv1 l)=> [] _ Hsym _. eauto.
+    move:(equiv1 l)=> [] _ _ Htrans. eauto.
 
-  -     ssa. de a0. de a1. de IRel. eauto.
-        de a1. de ORel. eauto.
 
-        ssa. de a. de IRel. eauto.
-        de ORel. eauto.
+    intros. de a0. de a1. de IRel;eauto. de IRel;eauto.
+    de ORel;eauto.
+    de a1. de ORel;eauto. de IRel;eauto. de ORel;eauto.
 
-        ssa. de a0. de a1. de IRel. eauto.
-        de a1. de ORel. eauto.
+
+    intros. de a. de IRel;eauto. de ORel;eauto.
+
+    intros. con.
+    intros. de a0. de a1. de a1.
+    de a0. de a1. eauto.
+    de a1. eauto.
 Defined.
 
 Definition levelPred := level -> Prop.
@@ -608,18 +735,31 @@ Definition eqmaybe_aux {V : Ty} (P: levelPred) (VRel : myrel [V]) : presP P -> m
 intros.  
     refine (@MyRel _
             (fun l v => if v is Some v' then dis VRel l v' else ~ P l)
-            (fun l b1 b2 => b1 = b2)
+            (fun l b1 b2 => b1 = b2 \/
+                              (if b1 is Some v' then dis VRel l v' else ~ P l) /\
+                               if b2 is Some v' then dis VRel l v' else ~ P l)
             _
             _
             _
             _).
-    intros. auto.
-ssa. de a.
-de VRel. eauto. intro. apply H1. apply/H. eauto. done.
-intros. de a0. de a1. inv H1. subst. done.
-subst. done.
-Defined.
+    intros. con.
+    intro. auto.
+    intro. intros. de H0.
+    intro. intros. de H0. de H1. subst. auto.
+    subst. de y. de x. de y. de H1. subst. auto.
+    de H1. subst. auto.
+    de H1. subst. auto.
 
+    intros. de H1. right.
+    de VRel. de a0. eauto. eauto. de a1. eauto. eauto.
+
+    intros. de VRel. de a. eauto. eauto.
+
+    intros. con.
+
+    intros. right. de a0.
+    intros. de H1. subst. done.
+Defined.    
 
 Definition Option_presP : presP (fun _ => True).
   rewrite /presP. eauto.
@@ -652,9 +792,9 @@ Defined.
 Fixpoint to_rel (ty : Ty): myrel [ty]:=
       match ty as x return myrel [x] with
     | TInput => publicRel TInput
-    | THandlerOutput => privateRel THandlerOutput
-    | TTypeSyscall => privateRel TTypeSyscall                                 
-    | TInterrupt => privateRel TInterrupt
+    | THandlerOutput => semiprivateRel THandlerOutput
+    | TTypeSyscall => semiprivateRel TTypeSyscall                                 
+    | TInterrupt => semiprivateRel TInterrupt
     | Option t => eqmaybe (to_rel t)
     | Option_swi t => eqmaybe_swi (to_rel t)
     | Option_maybe t => eqmaybe_maybe (to_rel t)
@@ -954,14 +1094,13 @@ Proof.
       exists o0. ssa. exists (@out _ _ o0). con. eauto. eauto.
 Qed.
 
+
 Lemma map_NI : forall (I I' O O' : Ty) (p : Proc I' O) (f : [I] -> [I']) (g : [O] -> [O']) (IRel : myrel [I]) (IRel' : myrel [I']) (ORel : myrel [O]) (ORel' : myrel [O']),
     NI IRel' ORel p -> 
     f_NI IRel IRel' f -> f_PU IRel IRel' f -> f_NI ORel ORel' g ->
     NI IRel ORel' (map f g p).
 Proof.
-  intros.
-  move: H. rewrite /NI. intros.
-  suff: simulation IRel' ORel l s p -> simulation IRel ORel' l s (map f g p).
+Admitted. 
 
 Lemma sta_NI : forall (I O V : Ty) (p : Proc (Times V I) O) f g v (IRel : myrel [I]) (VRel : myrel [V]) (ORel : myrel [O]),
     NI (eqpair_R VRel IRel) ORel p -> fv_NI ORel VRel VRel g -> fv_NI IRel VRel VRel f -> f_EP IRel VRel f -> NI IRel (eqpair VRel ORel) (sta f g v p).
@@ -1040,9 +1179,10 @@ Definition scheduled_p (I O : Ty) (b : bool) (p : Proc I O) :=
                     (maybe p))))).
 
 
-Lemma par_swiI_NI : forall (I1 I2 O1 O2 : Ty) (b : bool) (p1 : Proc I1 O1) (p2 : Proc I2 O2) (IRel1 : myrel [I1]) (IRel2 : myrel [I2]) (ORel1 : myrel [O1]) (ORel2 : myrel [O2]),
+(*Comment: Maybe prove this? We need it for example 2 (shows noninterference)*)
+(*Lemma par_swiI_NI : forall (I1 I2 O1 O2 : Ty) (b : bool) (p1 : Proc I1 O1) (p2 : Proc I2 O2) (IRel1 : myrel [I1]) (IRel2 : myrel [I2]) (ORel1 : myrel [O1]) (ORel2 : myrel [O2]),
      NI IRel1 ORel1 p1 -> NI IRel2 ORel2 p2 -> NI (eqpair_LR boolRel (eqpair IRel1 IRel2)) (eqpair (eqmaybe_swi ORel1) (eqmaybe_swi ORel2)) (par_swiI b p1 p2).
-Proof. Admitted.
+Proof. Admitted.*)
 
 (*sta_swi b n f p:
  (i == n,I') -> enables p
@@ -1086,17 +1226,16 @@ Definition streamType := Stream ([TInput] + (([ExOutputType]))).
 
 Definition OutputRel : myrel ([TOutput]).
   refine (@MyRel _
-            (fun l a => if l == \bot  then a = Step else False)
+            (fun l a => l = \bot /\ a = Step )
             (fun l a b => a = b) _ _ _ _).
   intros.
   done.
-  intros.
-  move: H0.
-  case_if;last by [].
-  rewrite /order (eqP H0) lex0 in H.
-  by rewrite H.
-
-  by intros;subst.
+  intros. ssa. subst. subst. subst.
+  Search _ order.
+  move/order_bot : H. move=>->. done.
+  intros. ssa. subst. con.
+  ssa.
+  ssa.
 Defined.
 
 Definition Output_option_presP : presP (fun l => l = \top).
@@ -1168,18 +1307,17 @@ Qed.
 
 Definition InputRel : myrel ([TInput]). 
   refine (@MyRel _
-            (fun l a => if l == \bot then a = DiskRead else False)
+            (fun l a => l = \bot /\ a = DiskRead)
             (fun l a b => a = b) _ _ _ _).
   intros.
   done.
-  intros.
-  move: H0.
-  case_if;last by [].
-  move: H. rewrite /order.
-  move/eqP: H0. intros. subst.
-  rewrite lex0 in H. rewrite H. done.
-  intros. subst. done.
-Defined.
+  intros. ssa. subst. subst. subst.
+  Search _ order.
+  move/order_bot : H. move=>->. done.
+  intros. ssa. subst. con.
+  ssa.
+  ssa.
+Defined.  
 
 (*NotSim*)
 Example counterexample : NotSim \bot InputRel (publicRel _) newtrace_simple (scheduler process_pool).
@@ -1188,7 +1326,7 @@ Proof.
   apply:NS4. ssa. de o'. subst.
   
   apply: NS2. instantiate (1:= (DiskRead)).
-  rewrite /= eqxx. auto.
+  ssa.
 
   intros. match_dd.
 
@@ -1209,46 +1347,137 @@ Proof.
 Qed.
 End Example1.
 
-(*Example 2: Non-interference
- round-robin between p_high and p_low
- input is public*)
-Module Example2.
-Definition p_high := (@out TInput TOutput Step). 
-Definition p_low := (@out TInput TOutput Idle). 
-Definition process_pool := par_swiI false p_high p_low.
-Definition scheduler {I O} (p : Proc (Times Bool (Times I I)) O) : Proc I O := @map _ (Times Bool (Times _ _)) _ _ (fun i => (true,(i,i))) id p.
-
-Definition InputRelPublic : myrel ([TInput]) := publicRel TInput. 
 
 Definition TraceF_specific := (@TraceF TInput (Times (Option TOutput) (Option TOutput))).
 Lemma specific_monotone : monotone2 TraceF_specific.
   apply (@monotone_TraceF TInput (Times (Option TOutput) (Option TOutput))).
 Qed.
-
 Hint Resolve specific_monotone : paco.
 
 
+
+
+Coercion to_rel_locked : Ty >-> myrel.
+
 Arguments NI : clear implicits.
-(*Arguments NI I O [_] [_].*)
-Example hl_lp_NI : @NI _ _ InputRelPublic (publicRel _) (scheduler process_pool).
+Arguments NI I O IRel ORel.
+Lemma NI_swap_rel : forall I O (p : Proc I O) (IRel : myrel [I]) (ORel ORel' : myrel [O]), (forall l x y, rel ORel l x y <-> rel ORel' l x y) -> NI I O IRel ORel p -> NI I O IRel ORel' p.
 Proof.
+  intros. intro. intros. eapply H0 in H1.
+  move: H1. instantiate (1:= l).
+  intros. apply/paco2_imp. apply monotone_SimulationF.
+  2:eauto. ssa.
+  inv H2;econ;eauto.
+  rewrite /Clause4. ssa. apply H6 in H7. ssa. exists x.
+  ssa;eauto. apply/H. done.
+Qed.  
+
+(*Lemma NI_add_L : forall I V O (p : Proc I (Times V O)) IRel,
+    NI I (Times V O) IRel (eqpair_R (to_rel V) (to_rel O)) p ->
+    NI I (Times V O) IRel (eqpair_LR (to_rel V) (to_rel O)) p.
+Proof.
+  intros. 
+  apply/simulation_equiv.
+  move/simulation_equiv : H.
+  intros. apply/NI_swap_rel. 2:eauto.
+  ssa.
+Qed.
+
+Lemma NI_add_R : forall I V O (p : Proc I (Times V O)) IRel,
+    NI I (Times V O) IRel (eqpair (to_rel V) (to_rel O)) p ->
+    NI I (Times V O) IRel (eqpair_R (to_rel V) (to_rel O)) p.
+Proof.
+  intros. 
+  apply/simulation_equiv.
+  move/simulation_equiv : H.
+  intros. apply/NI_swap_rel. 2:eauto.
+  ssa.
+Qed.*)
+
+Lemma SimulationF_I_imp : forall I O l (IRel IRel' : myrel [I]) (ORel : myrel [O]) R s p,
+    (forall l x, dis IRel' l x -> dis IRel l x) ->
+    (forall l x y, rel IRel l x y <-> rel IRel' l x y) ->
+    SimulationF l IRel ORel R s p ->
+    SimulationF l IRel' ORel R s p.
+Proof.
+  intros. inv H1. con;eauto.
+  rewrite /Clause1. ssa. eauto.
+  rewrite /Clause2. ssa. 
+  rewrite /Clause3. ssa.
+  move: H4. rewrite /Clause3. ssa. eapply H4 in H6;eauto. apply/H0. done.
+Qed.
+
+
+Lemma simulation_I_imp : forall I O (IRel IRel' : myrel [I]) (ORel : myrel [O]) p,
+    (forall l x, dis IRel' l x -> dis IRel l x) -> (forall l x y, rel IRel l x y <-> rel IRel' l x y) -> NI I O IRel ORel p -> NI I O IRel' ORel p.
+Proof.
+  intros. 
+  intros. rewrite /NI. intros. eapply H1 in H2.
+  move: H2. instantiate (1:=l).
+  apply:paco2_imp. apply monotone_SimulationF.
+  intros. apply/SimulationF_I_imp. 3:eauto. eauto. eauto.
+Qed.
+
+(*Lemma iNI_add_L : forall I V O (p : Proc (Times V I) O) VRel IRel ORel,
+    NI (Times V I) O (eqpair_R VRel IRel) ORel p ->
+    NI (Times V I) O (eqpair_LR VRel IRel) ORel p.
+Proof.
+  intros. 
+  apply/simulation_I_imp. 3:eauto.
+  ssa. ssa.
+Qed.*)
+
+
+(* Example removed for now. We can add it later if we prove NI for par_swiI
+  
+Example 2: Non-interference
+ round-robin between p_high and p_low
+ input is public*)
+(*Module Example2.
+Definition p_high := (@out TInput TOutput Step). 
+Definition p_low := (@out TInput TOutput Idle). 
+Definition process_pool := par_swiI false p_high p_low.
+Definition scheduler {I O} (p : Proc (Times Bool (Times I I)) O) : Proc I O := @map _ (Times Bool (Times _ _)) _ _ (fun i => (true,(i,i))) id p.
+
+
+Definition InputRel : myrel ([TInput]). 
+  refine (@MyRel _
+            (fun l a => l = \bot /\ a = DiskRead)
+            (fun l a b => a = b) _ _ _ _).
+  intros.
+  done.
+  intros. ssa. subst. subst. subst.
+  Search _ order.
+  move/order_bot : H. move=>->. done.
+  intros. ssa. subst. con.
+  ssa.
+  ssa.
+Defined.  
+(*Definition InputRelPublic : myrel ([TInput]) := publicRel TInput.*)
+
+Example hl_lp_NI : @NI TInput (Times (Option_swi TOutput) (Option_swi TOutput))
+                     InputRel (*InputRel*)
+                     (eqpair (eqmaybe_swi (publicRel TOutput)) (eqmaybe_swi (publicRel TOutput))) (*OutputRel*)
+                     (scheduler process_pool).
+Proof. simpl.
   rewrite /scheduler.
-  eapply map_NI. 
+  eapply map_NI.
   eapply par_swiI_NI.
   apply out_NI.
+  apply/simulation_I_imp. shelve. shelve.
   apply out_NI.
-  instantiate (1:= (InputRelPublic)).
-  instantiate (1:= (InputRelPublic)).  
-  rewrite /f_NI. ssa.
+  instantiate (1:= InputRel). instantiate (1:= InputRel).
+  intro. intros. ssa.
+  intro. intros. simpl in H. simpl. 
+  rewrite /f_NI. intros. rewrite /InputRel /= in H. simpl.
 
-  rewrite /f_PU. ssa.
-  rewrite /f_NI. ssa.
-  de i. de i'. by subst.
-  Unshelve. apply OutputRel. apply OutputRel.
+  rewrite /f_PU. ssa. simpl.
+  rewrite /f_NI. intros. eauto.
 Qed.
-End Example2.
+End Example2.*)
 
-Print Hint *. 
+
+
 (*Example 3
   Consists of two sub-examples (a) and (b)
   (a) round robin between low_p, high_p. Execution of either process is disrupted by hardware interrupt that schedules handler
@@ -1483,7 +1712,9 @@ apply: NS2.
                                                            This is a contradiction
                                                           *)
   ssa.
+  Print match_dd.
   match_dd.
+  eauto.
 Qed.
 
 Example example_not_NI : ~ @NI _ _ InputTypeRel OutputTypeRel (bad_scheduler process_pool).
@@ -1494,7 +1725,6 @@ Proof.
 Qed.
 
 (**** Example (b) ****)
-Coercion to_rel_locked : Ty >-> myrel.
 
 (*Definition NI2 I O (p : Proc I O) := NI I O I O p.
 Definition f_NI2 {I O :Ty} (f : [I] -> [O]) := forall (l : level) (i i' : [I]) (o o' : [O]), rel I l i i' -> rel O l (f i) (f i').
@@ -1520,71 +1750,7 @@ Qed.*)
 (*Lemma map_NI3 : forall (Ia Ib Ia' Ib' O O' : Ty) (p : Proc (Times Ia' Ib') O) (f : [Times Ia Ib] -> [Times Ia' Ib']) (g : [O] -> [O']), NI _ _ (eqpair_R Ia Ib) O (@map (Times _ _) (Times _ _) _ _ f g p).*)
 
 
-Lemma NI_swap_rel : forall I O (p : Proc I O) (IRel : myrel [I]) (ORel ORel' : myrel [O]), (forall l x y, rel ORel l x y <-> rel ORel' l x y) -> NI I O IRel ORel p -> NI I O IRel ORel' p.
-Proof.
-  intros. intro. intros. eapply H0 in H1.
-  move: H1. instantiate (1:= l).
-  intros. apply/paco2_imp. apply monotone_SimulationF.
-  2:eauto. ssa.
-  inv H2;econ;eauto.
-  rewrite /Clause4. ssa. apply H6 in H7. ssa. exists x.
-  ssa;eauto. apply/H. done.
-Qed.  
 
-Lemma NI_add_L : forall I V O (p : Proc I (Times V O)) IRel,
-    NI I (Times V O) IRel (eqpair_R (to_rel V) (to_rel O)) p ->
-    NI I (Times V O) IRel (eqpair_LR (to_rel V) (to_rel O)) p.
-Proof.
-  intros. 
-  apply/simulation_equiv.
-  move/simulation_equiv : H.
-  intros. apply/NI_swap_rel. 2:eauto.
-  ssa.
-Qed.
-
-Lemma NI_add_R : forall I V O (p : Proc I (Times V O)) IRel,
-    NI I (Times V O) IRel (eqpair (to_rel V) (to_rel O)) p ->
-    NI I (Times V O) IRel (eqpair_R (to_rel V) (to_rel O)) p.
-Proof.
-  intros. 
-  apply/simulation_equiv.
-  move/simulation_equiv : H.
-  intros. apply/NI_swap_rel. 2:eauto.
-  ssa.
-Qed.
-
-Lemma SimulationF_I_imp : forall I O l (IRel IRel' : myrel [I]) (ORel : myrel [O]) R s p,
-    (forall l x, dis IRel' l x -> dis IRel l x) ->
-    (forall l x y, rel IRel l x y <-> rel IRel' l x y) ->
-    SimulationF l IRel ORel R s p ->
-    SimulationF l IRel' ORel R s p.
-Proof.
-  intros. inv H1. con;eauto.
-  rewrite /Clause1. ssa. eauto.
-  rewrite /Clause2. ssa. 
-  rewrite /Clause3. ssa.
-  move: H4. rewrite /Clause3. ssa. eapply H4 in H6;eauto. apply/H0. done.
-Qed.
-
-
-Lemma simulation_I_imp : forall I O (IRel IRel' : myrel [I]) (ORel : myrel [O]) p,
-    (forall l x, dis IRel' l x -> dis IRel l x) -> (forall l x y, rel IRel l x y <-> rel IRel' l x y) -> NI I O IRel ORel p -> NI I O IRel' ORel p.
-Proof.
-  intros. 
-  intros. rewrite /NI. intros. eapply H1 in H2.
-  move: H2. instantiate (1:=l).
-  apply:paco2_imp. apply monotone_SimulationF.
-  intros. apply/SimulationF_I_imp. 3:eauto. eauto. eauto.
-Qed.
-
-Lemma iNI_add_L : forall I V O (p : Proc (Times V I) O) VRel IRel ORel,
-    NI (Times V I) O (eqpair_R VRel IRel) ORel p ->
-    NI (Times V I) O (eqpair_LR VRel IRel) ORel p.
-Proof.
-  intros. 
-  apply/simulation_I_imp. 3:eauto.
-  ssa. ssa.
-Qed.
 
 (*Lemma iNI_to_LR_boolRel : forall I O (p : Proc (Times Bool I) O) IRel ORel,
     NI (Times Bool I) O (eqpair_LR boolRel IRel) ORel p ->
